src/x86/instrrules/cmp.v
@@ -40,7 +40,7 @@ Qed.
 End setoid_rewrite_opacity.
 
 Ltac basicCMP_ZC :=
-  rewrite /makeBOP; 
+  rewrite /makeBOP/UOPArgM4/BOPArgI4; 
   let R := lazymatch goal with
              | |- |-- basic ?p (@BOP ?d OP_CMP ?a) ?O ?q => constr:(@CMP_ruleZC d a)
            end in
@@ -103,10 +103,10 @@ Lemma CMP_RR_rule (r1 r2:GPReg32) v1 (v2:DWORD):
 Proof. basic apply *. Qed.
 
 
-Lemma CMP_RI_ZC_rule (r1:GPReg32) v1 (v2:VWORD OpSize4):
+Lemma CMP_RI_ZC_rule (r1:GPReg32) v1 (v2:DWORD):
   |-- basic (r1 ~= v1 ** OSZCP?) (CMP r1, v2) empOP
             (r1 ~= v1 ** OF? ** SF? ** PF? ** CF ~= ltB v1 v2 ** ZF ~= (v1==v2)).
-Proof. unfold makeBOP, VWORDasIMM. basicCMP_ZC. Qed.
+Proof. basicCMP_ZC. Qed.
 
 (*
 Lemma CMP_MbR_ZC_rule (r1:GPReg32) (r2: Reg8) (p:DWORD) (v1 v2:BYTE):
