src/x86/instrsyntax.v
@@ -22,11 +22,6 @@ Definition fromSingletonMemSpec seg (msa: SingletonMemSpec) :=
   | RegMemSpec r => mkMemSpec AdSize4 seg (Some (mkSIB _ r None)) (natAsDWORD 0)
   end.
 
-Inductive InstrArg s :=
-| InstrArgR (r: GPReg s) :> InstrArg s 
-| InstrArgM a (m:MemSpec a) : InstrArg s
-| InstrArgI (v: VWORD s) :> InstrArg s.
-
 Definition VWORDasIMM s : VWORD s -> option (IMM s) :=
   match s with
   | OpSize1 => fun x => Some x
@@ -36,93 +31,60 @@ Definition VWORDasIMM s : VWORD s -> option (IMM s) :=
   end.
 
 Notation "'[' m ']'" :=
-  (InstrArgM _ _ (fromSingletonMemSpec None m))
+  (fromSingletonMemSpec None m)
   (at level 0, m at level 0) : memspec_scope.
 
 Notation "s ':[' m ']'" :=
-  (InstrArgM _ _ (fromSingletonMemSpec (Some s) m))
+  (fromSingletonMemSpec (Some s) m)
   (at level 1, m at level 0) : memspec_scope.
 
 Notation "'[' r '+' n ']'" :=
-  (InstrArgM _ _ (mkMemSpec _ None (Some(mkSIB _ (r:BaseReg _) None)) n))
+  (mkMemSpec _ None (Some(mkSIB _ (r:BaseReg _) None)) n)
   (at level 0, r at level 0, n at level 0) : memspec_scope.
 
 Notation "s ':[' r '+' n ']'" :=
-  (InstrArgM _ _ (mkMemSpec _ (Some s) (Some(mkSIB _ (r:BaseReg _) None)) n))
+  (mkMemSpec _ (Some s) (Some(mkSIB _ (r:BaseReg _) None)) n)
   (at level 1, r at level 0, n at level 0, format "s :[ r + n ] ") : memspec_scope.
 
 Notation "'[' r '-' n ']'" :=
-  (InstrArgM _ _ (mkMemSpec _ None (Some(mkSIB _ (r:BaseReg _) None)) (negB n)))
+  (mkMemSpec _ None (Some(mkSIB _ (r:BaseReg _) None)) (negB n))
   (at level 0, r at level 0, n at level 0) : memspec_scope.
 
 Notation "s ':[' r '-' n ']'" :=
-  (InstrArgM _ _ (mkMemSpec _ (Some s) (Some(mkSIB _ (r:BaseReg _) None)) (negB n)))
+  (mkMemSpec _ (Some s) (Some(mkSIB _ (r:BaseReg _) None)) (negB n))
   (at level 1, r at level 0, n at level 0, format "s :[ r - n ] ") : memspec_scope.
 
 Notation "'[' r '+' i '+' n ']'" :=
-  (InstrArgM _ _ (mkMemSpec _ None (Some(mkSIB _ (r:BaseReg _) (Some (i,S1)))) n))
+  (mkMemSpec _ None (Some(mkSIB _ (r:BaseReg _) (Some (i,S1)))) n)
   (at level 0, r at level 0, i at level 0, n at level 0) : memspec_scope.
 
 Notation "s ':[' r '+' i '+' n ']'" :=
-  (InstrArgM _ _ (mkMemSpec _ (Some s) (Some(mkSIB _ (r:BaseReg _) (Some (i,S1)))) n))
+  (mkMemSpec _ (Some s) (Some(mkSIB _ (r:BaseReg _) (Some (i,S1)))) n)
   (at level 1, r at level 0, i at level 0, n at level 0, format "s :[ r + i + n ]") : memspec_scope.
 
 Notation "'[' r '+' i '*' '2' ']'" :=
-  (InstrArgM _ _ (mkMemSpec _ None (Some(mkSIB _ (r:BaseReg _) (Some(i,S2)))) #0))
+  (mkMemSpec _ None (Some(mkSIB _ (r:BaseReg _) (Some(i,S2)))) #0)
   (at level 0, r at level 0, i at level 0) : instr_scope.
 
 Notation "'[' r '+' i '*' '2' '+' n ']'" :=
-  (InstrArgM _ _ (mkMemSpec _ None (Some(mkSIB _ (r:BaseReg _) (Some(i,S2)))) n))
+  (mkMemSpec _ None (Some(mkSIB _ (r:BaseReg _) (Some(i,S2)))) n)
   (at level 0, r at level 0, i at level 0, n at level 0) : memspec_scope.
 
 Notation "'[' r '+' i '*' '4' ']'" :=
-  (InstrArgM _ _ (mkMemSpec _ None (Some(mkSIB _ (r:BaseReg _) (Some(i,S4)))) 0))
+  (mkMemSpec _ None (Some(mkSIB _ (r:BaseReg _) (Some(i,S4)))) 0)
   (at level 0, r at level 0, i at level 0) : instr_scope.
 
 Notation "'[' r '+' i '*' '4' '+' n ']'" :=
-  (InstrArgM _ _ (mkMemSpec _ None (Some(mkSIB _ (r:BaseReg _) (Some(i,S4)))) n))
+  (mkMemSpec _ None (Some(mkSIB _ (r:BaseReg _) (Some(i,S4)))) n)
   (at level 0, r at level 0, i at level 0, n at level 0) : memspec_scope.
 
 Notation "'[' r '+' i '*' '8' ']'" :=
-  (InstrArgM _ _ (mkMemSpec _ None (Some(mkSIB _ (r:BaseReg _) (Some(i,S8)))) 0))
+  (mkMemSpec _ None (Some(mkSIB _ (r:BaseReg _) (Some(i,S8)))) 0)
   (at level 0, r at level 0, i at level 0) : instr_scope.
 
 Notation "'[' r '+' i '*' '8' '+' n ']'" :=
-  (InstrArgM _ _ (mkMemSpec _ None (Some(mkSIB _ (r:BaseReg _) (Some(i,S8)))) n))
+  (mkMemSpec _ None (Some(mkSIB _ (r:BaseReg _) (Some(i,S8)))) n)
   (at level 0, r at level 0, i at level 0, n at level 0) : memspec_scope.
-
-(*---------------------------------------------------------------------------
-    Binary operations
-  ---------------------------------------------------------------------------*)
-Definition makeBOP s op dst (src: InstrArg s) :=
-  match dst, src with
-  | InstrArgR dst, InstrArgR src => BOP s op (DstSrcRR s dst src)
-  | InstrArgR dst, InstrArgM a src => BOP s op (DstSrcRM s a dst src)
-
-  | InstrArgR dst, InstrArgI n => 
-    if VWORDasIMM s n is Some v then BOP s op (DstSrcRI s dst v) 
-    else BADINSTR
-
-  | InstrArgM a dst, InstrArgR src => BOP s op (DstSrcMR s a dst src)
-  | InstrArgM a dst, InstrArgI n => 
-    if VWORDasIMM s n is Some v then BOP s op (DstSrcMI s a dst v) 
-    else BADINSTR
-    
-  | _, _=> BADINSTR
-  end.
-
-Definition makeUOP s op (arg: InstrArg s) :=
-  match arg with
-  | InstrArgR r => UOP _ op (RegMemR s r)
-  | InstrArgM a m => UOP _ op (RegMemM s a m)
-  | _ => BADINSTR
-  end.
-
-Definition makeLEA s r (arg: InstrArg s) :=
-  match arg with
-  | InstrArgM a m => LEA s r (RegMemM s a m)
-  | _ => BADINSTR
-  end.
 
 Open Scope instr_scope.
 
@@ -131,85 +93,279 @@ Bind Scope memspec_scope with MemSpec.
 (*---------------------------------------------------------------------------
     Unary operations
   ---------------------------------------------------------------------------*)
+Inductive UOPArg s :=
+| UOPArgR (r: GPReg s) :> UOPArg s 
+| UOPArgM a (m:MemSpec a) : UOPArg s.
+
+Coercion UOPArgM4 a (m: MemSpec a) : UOPArg OpSize4 := UOPArgM OpSize4 a m.
+
+Definition makeUOP s op (arg: UOPArg s) :=
+  match arg with
+  | UOPArgR r => UOP _ op (RegMemR s r)
+  | UOPArgM a m => UOP _ op (RegMemM s a m)
+  end.
+
 Notation "'NOT' x"
   := (makeUOP _ OP_NOT x%ms) (x at level 55, at level 60) : instr_scope.
 Notation "'NOT' 'BYTE' 'PTR' m"
-  := (makeUOP OpSize1 OP_NOT m%ms) (m at level 55, at level 60) : instr_scope.
+  := (UOP OpSize1 OP_NOT (RegMemM _ _ m%ms)) (m at level 55, at level 60) : instr_scope.
 Notation "'NOT' 'WORD' 'PTR' m"
-  := (makeUOP OpSize2 OP_NOT m%ms) (m at level 55, at level 60) : instr_scope.
+  := (UOP OpSize2 OP_NOT (RegMemM _ _ m%ms)) (m at level 55, at level 60) : instr_scope.
 Notation "'NOT' 'DWORD' 'PTR' m"
-  := (makeUOP OpSize4 OP_NOT m%ms) (m at level 55, at level 60) : instr_scope.
+  := (UOP OpSize4 OP_NOT (RegMemM _ _ m%ms)) (m at level 55, at level 60) : instr_scope.
 Notation "'NOT' 'QWORD' 'PTR' m"
-  := (makeUOP OpSize8 OP_NOT m%ms) (m at level 55, at level 60) : instr_scope.
+  := (UOP OpSize8 OP_NOT (RegMemM _ _ m%ms)) (m at level 55, at level 60) : instr_scope.
+
+Example exNOT1 := NOT WORD PTR [EBX+4].
+Example exNOT2 := NOT [EBX+ECX*4+9].
+Example exNOT3 := NOT CL. 
 
 Notation "'NEG' x"
   := (makeUOP _ OP_NEG x%ms) (x at level 55, at level 60) : instr_scope.
 Notation "'NEG' 'BYTE' 'PTR' m"
-  := (makeUOP OpSize1 OP_NEG m%ms) (m at level 55, at level 60) : instr_scope.
+  := (UOP OpSize1 OP_NEG (RegMemM _ _ m%ms)) (m at level 55, at level 60) : instr_scope.
 Notation "'NEG' 'WORD' 'PTR' m"
-  := (makeUOP OpSize2 OP_NEG m%ms) (m at level 55, at level 60) : instr_scope.
+  := (UOP OpSize2 OP_NEG (RegMemM _ _ m%ms)) (m at level 55, at level 60) : instr_scope.
 Notation "'NEG' 'DWORD' 'PTR' m"
-  := (makeUOP OpSize4 OP_NEG m%ms) (m at level 55, at level 60) : instr_scope.
+  := (UOP OpSize4 OP_NEG (RegMemM _ _ m%ms)) (m at level 55, at level 60) : instr_scope.
 Notation "'NEG' 'QWORD' 'PTR' m"
-  := (makeUOP OpSize8 OP_NEG m%ms) (m at level 55, at level 60) : instr_scope.
+  := (UOP OpSize8 OP_NEG (RegMemM _ _ m%ms)) (m at level 55, at level 60) : instr_scope.
+
+Example exNEG1 := NEG [EDI].
 
 Notation "'INC' x"
   := (makeUOP _ OP_INC x%ms) (x at level 55, at level 60) : instr_scope.
 Notation "'INC' 'BYTE' 'PTR' m"
-  := (makeUOP OpSize1 OP_INC m%ms) (m at level 55, at level 60) : instr_scope.
+  := (UOP OpSize1 OP_INC (RegMemM _ _ m%ms)) (m at level 55, at level 60) : instr_scope.
 Notation "'INC' 'WORD' 'PTR' m"
-  := (makeUOP OpSize2 OP_INC m%ms) (m at level 55, at level 60) : instr_scope.
+  := (UOP OpSize2 OP_INC (RegMemM _ _ m%ms)) (m at level 55, at level 60) : instr_scope.
 Notation "'INC' 'DWORD' 'PTR' m"
-  := (makeUOP OpSize4 OP_INC m%ms) (m at level 55, at level 60) : instr_scope.
+  := (UOP OpSize4 OP_INC (RegMemM _ _ m%ms)) (m at level 55, at level 60) : instr_scope.
 Notation "'INC' 'QWORD' 'PTR' m"
-  := (makeUOP OpSize8 OP_INC m%ms) (m at level 55, at level 60) : instr_scope.
+  := (UOP OpSize8 OP_INC (RegMemM _ _ m%ms)) (m at level 55, at level 60) : instr_scope.
+
+Example exINC1 := INC [EAX+ESI*4].
+Example exINC2 := INC R12.
+Example exINC3 := INC BYTE PTR [ECX + EDI*4 + 78].
 
 Notation "'DEC' x"
   := (makeUOP _ OP_DEC x%ms) (x at level 55, at level 60) : instr_scope.
 Notation "'DEC' 'BYTE' 'PTR' m"
-  := (makeUOP OpSize1 OP_DEC m%ms) (m at level 55, at level 60) : instr_scope.
+  := (UOP OpSize1 OP_DEC (RegMemM _ _ m%ms)) (m at level 55, at level 60) : instr_scope.
 Notation "'DEC' 'WORD' 'PTR' m"
-  := (makeUOP OpSize2 OP_DEC m%ms) (m at level 55, at level 60) : instr_scope.
+  := (UOP OpSize2 OP_DEC (RegMemM _ _ m%ms)) (m at level 55, at level 60) : instr_scope.
 Notation "'DEC' 'DWORD' 'PTR' m"
-  := (makeUOP OpSize4 OP_DEC m%ms) (m at level 55, at level 60) : instr_scope.
+  := (UOP OpSize4 OP_DEC (RegMemM _ _ m%ms)) (m at level 55, at level 60) : instr_scope.
 Notation "'DEC' 'QWORD' 'PTR' m"
-  := (makeUOP OpSize8 OP_DEC m%ms) (m at level 55, at level 60) : instr_scope.
+  := (UOP OpSize8 OP_DEC (RegMemM _ _ m%ms)) (m at level 55, at level 60) : instr_scope.
+
+Example exDEC1 := INC DWORD PTR [ECX + EDI*4 + 78].
+
+(*---------------------------------------------------------------------------
+    Binary operations
+  ---------------------------------------------------------------------------*)
+Inductive BOPArg s :=
+| BOPArgR (r: GPReg s) :> BOPArg s 
+| BOPArgM a (m:MemSpec a) : BOPArg s
+| BOPArgI (x: IMM s) :> BOPArg s. 
+
+Coercion BOPArgM4 a (m: MemSpec a) : BOPArg OpSize4 := BOPArgM OpSize4 a m.
+Coercion BOPArgI1 (x: BYTE) : BOPArg OpSize1 := BOPArgI OpSize1 x.
+Coercion BOPArgI2 (x: WORD) : BOPArg OpSize2 := BOPArgI OpSize2 x.
+Coercion BOPArgI4 (x: DWORD) : BOPArg OpSize4 := BOPArgI OpSize4 x.
+
+Definition makeBOP s op dst (src: BOPArg s) :=
+  match dst, src with
+  | UOPArgR dst, BOPArgR src => BOP s op (DstSrcRR s dst src)
+  | UOPArgR dst, BOPArgM a src => BOP s op (DstSrcRM s a dst src)
+
+  | UOPArgR dst, BOPArgI v => BOP s op (DstSrcRI s dst v) 
+
+  | UOPArgM a dst, BOPArgR src => BOP s op (DstSrcMR s a dst src)
+  | UOPArgM a dst, BOPArgI v =>  BOP s op (DstSrcMI s a dst v) 
+    
+  | _, _=> BADINSTR
+  end.
 
 Notation "'ADC' x , y" := (makeBOP _ OP_ADC x%ms y%ms) (x,y at level 55, at level 60) : instr_scope.
 Notation "'ADC' 'BYTE' 'PTR' x , y" :=
-  (makeBOP OpSize1 OP_ADC x%ms y) (x,y at level 55, at level 60) : instr_scope.
-Notation "'ADD' x , y" := (makeBOP _ OP_ADD x%ms y%ms) (x,y at level 56, at level 60) : instr_scope.
+  (makeBOP OpSize1 OP_ADC (UOPArgM _ _ x%ms) y) (x,y at level 55, at level 60) : instr_scope.
+Notation "'ADC' 'WORD' 'PTR' x , y" :=
+  (makeBOP OpSize2 OP_ADC (UOPArgM _ _ x%ms) y) (x,y at level 55, at level 60) : instr_scope.
+Notation "'ADC' 'DWORD' 'PTR' x , y" :=
+  (makeBOP OpSize4 OP_ADC (UOPArgM _ _ x%ms) y) (x,y at level 55, at level 60) : instr_scope.
+Notation "'ADC' 'QWORD' 'PTR' x , y" :=
+  (makeBOP OpSize8 OP_ADC (UOPArgM _ _ x%ms) y) (x,y at level 55, at level 60) : instr_scope.
+Notation "'ADC' x , 'BYTE' 'PTR' y" :=
+  (makeBOP OpSize1 OP_ADC x (BOPArgM _ _ y%ms)) (x,y at level 55, at level 60) : instr_scope.
+Notation "'ADC' x , 'WORD' 'PTR' y" :=
+  (makeBOP OpSize2 OP_ADC x (BOPArgM _ _ y%ms)) (x,y at level 55, at level 60) : instr_scope.
+Notation "'ADC' x , 'DWORD' 'PTR' y" :=
+  (makeBOP OpSize4 OP_ADC x (BOPArgM _ _ y%ms)) (x,y at level 55, at level 60) : instr_scope.
+Notation "'ADC' x , 'QWORD' 'PTR' y" :=
+  (makeBOP OpSize8 OP_ADC x (BOPArgM _ _ y%ms)) (x,y at level 55, at level 60) : instr_scope.
+Example exADC1 (x:DWORD) := ADC [EDI], x.
+Example exADC2 (x:WORD) := ADC WORD PTR [EDI], x.
+Example exADC3 := ADC R10, QWORD PTR [R12 + 4].
+Example exADC4 := ADC EAX, [EDI + 4].
+Example exADC5 := ADC BL, 10.
+Example exADC6 := ADC EAX, (10:DWORD).
+
+Notation "'ADD' x , y" := (makeBOP _ OP_ADD x%ms y%ms) (x,y at level 55, at level 60) : instr_scope.
 Notation "'ADD' 'BYTE' 'PTR' x , y" :=
-  (makeBOP OpSize1 OP_ADD x%ms y) (x,y at level 55, at level 60) : instr_scope.
+  (makeBOP OpSize1 OP_ADD (UOPArgM _ _ x%ms) y) (x,y at level 55, at level 60) : instr_scope.
+Notation "'ADD' 'WORD' 'PTR' x , y" :=
+  (makeBOP OpSize2 OP_ADD (UOPArgM _ _ x%ms) y) (x,y at level 55, at level 60) : instr_scope.
+Notation "'ADD' 'DWORD' 'PTR' x , y" :=
+  (makeBOP OpSize4 OP_ADD (UOPArgM _ _ x%ms) y) (x,y at level 55, at level 60) : instr_scope.
+Notation "'ADD' 'QWORD' 'PTR' x , y" :=
+  (makeBOP OpSize8 OP_ADD (UOPArgM _ _ x%ms) y) (x,y at level 55, at level 60) : instr_scope.
+Notation "'ADD' x , 'BYTE' 'PTR' y" :=
+  (makeBOP OpSize1 OP_ADD x (BOPArgM _ _ y%ms)) (x,y at level 55, at level 60) : instr_scope.
+Notation "'ADD' x , 'WORD' 'PTR' y" :=
+  (makeBOP OpSize2 OP_ADD x (BOPArgM _ _ y%ms)) (x,y at level 55, at level 60) : instr_scope.
+Notation "'ADD' x , 'DWORD' 'PTR' y" :=
+  (makeBOP OpSize4 OP_ADD x (BOPArgM _ _ y%ms)) (x,y at level 55, at level 60) : instr_scope.
+Notation "'ADD' x , 'QWORD' 'PTR' y" :=
+  (makeBOP OpSize8 OP_ADD x (BOPArgM _ _ y%ms)) (x,y at level 55, at level 60) : instr_scope.
+
+Example exADD1 := ADD EAX, [EBX + 3].
+Example exADD2 := ADD EBX, (12:DWORD).
+Example exADD3 := ADD WORD PTR [EBX], CX.
+Example exADD4 := ADD R10, QWORD PTR [R13 + 6].
+Example exADD5 := ADD R10, ((12:DWORD):IMM OpSize8).
+
 Notation "'SUB' x , y" := (makeBOP _ OP_SUB x%ms y%ms) (x,y at level 55, at level 60) : instr_scope.
 Notation "'SUB' 'BYTE' 'PTR' x , y" :=
-  (makeBOP OpSize1 OP_SUB x%ms y) (x,y at level 55, at level 60) : instr_scope.
+  (makeBOP OpSize1 OP_SUB (UOPArgM _ _ x%ms) y) (x,y at level 55, at level 60) : instr_scope.
+Notation "'SUB' 'WORD' 'PTR' x , y" :=
+  (makeBOP OpSize2 OP_SUB (UOPArgM _ _ x%ms) y) (x,y at level 55, at level 60) : instr_scope.
+Notation "'SUB' 'DWORD' 'PTR' x , y" :=
+  (makeBOP OpSize4 OP_SUB (UOPArgM _ _ x%ms) y) (x,y at level 55, at level 60) : instr_scope.
+Notation "'SUB' 'QWORD' 'PTR' x , y" :=
+  (makeBOP OpSize8 OP_SUB (UOPArgM _ _ x%ms) y) (x,y at level 55, at level 60) : instr_scope.
+Notation "'SUB' x , 'BYTE' 'PTR' y" :=
+  (makeBOP OpSize1 OP_SUB x (BOPArgM _ _ y%ms)) (x,y at level 55, at level 60) : instr_scope.
+Notation "'SUB' x , 'WORD' 'PTR' y" :=
+  (makeBOP OpSize2 OP_SUB x (BOPArgM _ _ y%ms)) (x,y at level 55, at level 60) : instr_scope.
+Notation "'SUB' x , 'DWORD' 'PTR' y" :=
+  (makeBOP OpSize4 OP_SUB x (BOPArgM _ _ y%ms)) (x,y at level 55, at level 60) : instr_scope.
+Notation "'SUB' x , 'QWORD' 'PTR' y" :=
+  (makeBOP OpSize8 OP_SUB x (BOPArgM _ _ y%ms)) (x,y at level 55, at level 60) : instr_scope.
+
 Notation "'SBB' x , y" := (makeBOP _ OP_SBB x%ms y%ms) (x,y at level 55, at level 60) : instr_scope.
 Notation "'SBB' 'BYTE' 'PTR' x , y" :=
-  (makeBOP OpSize1 OP_SBB x%ms y) (x,y at level 55, at level 60) : instr_scope.
+  (makeBOP OpSize1 OP_SBB (UOPArgM _ _ x%ms) y) (x,y at level 55, at level 60) : instr_scope.
+Notation "'SBB' 'WORD' 'PTR' x , y" :=
+  (makeBOP OpSize2 OP_SBB (UOPArgM _ _ x%ms) y) (x,y at level 55, at level 60) : instr_scope.
+Notation "'SBB' 'DWORD' 'PTR' x , y" :=
+  (makeBOP OpSize4 OP_SBB (UOPArgM _ _ x%ms) y) (x,y at level 55, at level 60) : instr_scope.
+Notation "'SBB' 'QWORD' 'PTR' x , y" :=
+  (makeBOP OpSize8 OP_SBB (UOPArgM _ _ x%ms) y) (x,y at level 55, at level 60) : instr_scope.
+Notation "'SBB' x , 'BYTE' 'PTR' y" :=
+  (makeBOP OpSize1 OP_SBB x (BOPArgM _ _ y%ms)) (x,y at level 55, at level 60) : instr_scope.
+Notation "'SBB' x , 'WORD' 'PTR' y" :=
+  (makeBOP OpSize2 OP_SBB x (BOPArgM _ _ y%ms)) (x,y at level 55, at level 60) : instr_scope.
+Notation "'SBB' x , 'DWORD' 'PTR' y" :=
+  (makeBOP OpSize4 OP_SBB x (BOPArgM _ _ y%ms)) (x,y at level 55, at level 60) : instr_scope.
+Notation "'SBB' x , 'QWORD' 'PTR' y" :=
+  (makeBOP OpSize8 OP_SBB x (BOPArgM _ _ y%ms)) (x,y at level 55, at level 60) : instr_scope.
+
+
 Notation "'AND' x , y" := (makeBOP _ OP_AND x%ms y%ms) (x,y at level 55, at level 60) : instr_scope.
 Notation "'AND' 'BYTE' 'PTR' x , y" :=
-  (makeBOP OpSize1 OP_AND x%ms y) (x,y at level 55, at level 60) : instr_scope.
+  (makeBOP OpSize1 OP_AND (UOPArgM _ _ x%ms) y) (x,y at level 55, at level 60) : instr_scope.
+Notation "'AND' 'WORD' 'PTR' x , y" :=
+  (makeBOP OpSize2 OP_AND (UOPArgM _ _ x%ms) y) (x,y at level 55, at level 60) : instr_scope.
+Notation "'AND' 'DWORD' 'PTR' x , y" :=
+  (makeBOP OpSize4 OP_AND (UOPArgM _ _ x%ms) y) (x,y at level 55, at level 60) : instr_scope.
+Notation "'AND' 'QWORD' 'PTR' x , y" :=
+  (makeBOP OpSize8 OP_AND (UOPArgM _ _ x%ms) y) (x,y at level 55, at level 60) : instr_scope.
+Notation "'AND' x , 'BYTE' 'PTR' y" :=
+  (makeBOP OpSize1 OP_AND x (BOPArgM _ _ y%ms)) (x,y at level 55, at level 60) : instr_scope.
+Notation "'AND' x , 'WORD' 'PTR' y" :=
+  (makeBOP OpSize2 OP_AND x (BOPArgM _ _ y%ms)) (x,y at level 55, at level 60) : instr_scope.
+Notation "'AND' x , 'DWORD' 'PTR' y" :=
+  (makeBOP OpSize4 OP_AND x (BOPArgM _ _ y%ms)) (x,y at level 55, at level 60) : instr_scope.
+Notation "'AND' x , 'QWORD' 'PTR' y" :=
+  (makeBOP OpSize8 OP_AND x (BOPArgM _ _ y%ms)) (x,y at level 55, at level 60) : instr_scope.
+
 Notation "'OR' x , y" := (makeBOP _ OP_OR x%ms y%ms) (x,y at level 55, at level 60) : instr_scope.
 Notation "'OR' 'BYTE' 'PTR' x , y" :=
-  (makeBOP OpSize1 OP_OR x%ms y) (x,y at level 55, at level 60) : instr_scope.
+  (makeBOP OpSize1 OP_OR (UOPArgM _ _ x%ms) y) (x,y at level 55, at level 60) : instr_scope.
+Notation "'OR' 'WORD' 'PTR' x , y" :=
+  (makeBOP OpSize2 OP_OR (UOPArgM _ _ x%ms) y) (x,y at level 55, at level 60) : instr_scope.
+Notation "'OR' 'DWORD' 'PTR' x , y" :=
+  (makeBOP OpSize4 OP_OR (UOPArgM _ _ x%ms) y) (x,y at level 55, at level 60) : instr_scope.
+Notation "'OR' 'QWORD' 'PTR' x , y" :=
+  (makeBOP OpSize8 OP_OR (UOPArgM _ _ x%ms) y) (x,y at level 55, at level 60) : instr_scope.
+Notation "'OR' x , 'BYTE' 'PTR' y" :=
+  (makeBOP OpSize1 OP_OR x (BOPArgM _ _ y%ms)) (x,y at level 55, at level 60) : instr_scope.
+Notation "'OR' x , 'WORD' 'PTR' y" :=
+  (makeBOP OpSize2 OP_OR x (BOPArgM _ _ y%ms)) (x,y at level 55, at level 60) : instr_scope.
+Notation "'OR' x , 'DWORD' 'PTR' y" :=
+  (makeBOP OpSize4 OP_OR x (BOPArgM _ _ y%ms)) (x,y at level 55, at level 60) : instr_scope.
+Notation "'OR' x , 'QWORD' 'PTR' y" :=
+  (makeBOP OpSize8 OP_OR x (BOPArgM _ _ y%ms)) (x,y at level 55, at level 60) : instr_scope.
+
+
 Notation "'XOR' x , y" := (makeBOP _ OP_XOR x%ms y%ms) (x,y at level 55, at level 60) : instr_scope.
 Notation "'XOR' 'BYTE' 'PTR' x , y" :=
-  (makeBOP OpSize1 OP_XOR x%ms y) (x,y at level 55, at level 60) : instr_scope.
+  (makeBOP OpSize1 OP_XOR (UOPArgM _ _ x%ms) y) (x,y at level 55, at level 60) : instr_scope.
+Notation "'XOR' 'WORD' 'PTR' x , y" :=
+  (makeBOP OpSize2 OP_XOR (UOPArgM _ _ x%ms) y) (x,y at level 55, at level 60) : instr_scope.
+Notation "'XOR' 'DWORD' 'PTR' x , y" :=
+  (makeBOP OpSize4 OP_XOR (UOPArgM _ _ x%ms) y) (x,y at level 55, at level 60) : instr_scope.
+Notation "'XOR' 'QWORD' 'PTR' x , y" :=
+  (makeBOP OpSize8 OP_XOR (UOPArgM _ _ x%ms) y) (x,y at level 55, at level 60) : instr_scope.
+Notation "'XOR' x , 'BYTE' 'PTR' y" :=
+  (makeBOP OpSize1 OP_XOR x (BOPArgM _ _ y%ms)) (x,y at level 55, at level 60) : instr_scope.
+Notation "'XOR' x , 'WORD' 'PTR' y" :=
+  (makeBOP OpSize2 OP_XOR x (BOPArgM _ _ y%ms)) (x,y at level 55, at level 60) : instr_scope.
+Notation "'XOR' x , 'DWORD' 'PTR' y" :=
+  (makeBOP OpSize4 OP_XOR x (BOPArgM _ _ y%ms)) (x,y at level 55, at level 60) : instr_scope.
+Notation "'XOR' x , 'QWORD' 'PTR' y" :=
+  (makeBOP OpSize8 OP_XOR x (BOPArgM _ _ y%ms)) (x,y at level 55, at level 60) : instr_scope.
+
+
 Notation "'CMP' x , y" := (makeBOP _ OP_CMP x%ms y%ms) (x,y at level 55, at level 60) : instr_scope.
 Notation "'CMP' 'BYTE' 'PTR' x , y" :=
-  (makeBOP OpSize1 OP_CMP x%ms y) (x,y at level 55, at level 60) : instr_scope.
+  (makeBOP OpSize1 OP_CMP (UOPArgM _ _ x%ms) y) (x,y at level 55, at level 60) : instr_scope.
+Notation "'CMP' 'WORD' 'PTR' x , y" :=
+  (makeBOP OpSize2 OP_CMP (UOPArgM _ _ x%ms) y) (x,y at level 55, at level 60) : instr_scope.
+Notation "'CMP' 'DWORD' 'PTR' x , y" :=
+  (makeBOP OpSize4 OP_CMP (UOPArgM _ _ x%ms) y) (x,y at level 55, at level 60) : instr_scope.
+Notation "'CMP' 'QWORD' 'PTR' x , y" :=
+  (makeBOP OpSize8 OP_CMP (UOPArgM _ _ x%ms) y) (x,y at level 55, at level 60) : instr_scope.
+Notation "'CMP' x , 'BYTE' 'PTR' y" :=
+  (makeBOP OpSize1 OP_CMP x (BOPArgM _ _ y%ms)) (x,y at level 55, at level 60) : instr_scope.
+Notation "'CMP' x , 'WORD' 'PTR' y" :=
+  (makeBOP OpSize2 OP_CMP x (BOPArgM _ _ y%ms)) (x,y at level 55, at level 60) : instr_scope.
+Notation "'CMP' x , 'DWORD' 'PTR' y" :=
+  (makeBOP OpSize4 OP_CMP x (BOPArgM _ _ y%ms)) (x,y at level 55, at level 60) : instr_scope.
+Notation "'CMP' x , 'QWORD' 'PTR' y" :=
+  (makeBOP OpSize8 OP_CMP x (BOPArgM _ _ y%ms)) (x,y at level 55, at level 60) : instr_scope.
+
+
+Example exCMP1 := CMP BYTE PTR [EDI + ECX*2], (#c"*":IMM OpSize1).
 
 (*---------------------------------------------------------------------------
     MOV operations
   ---------------------------------------------------------------------------*)
-Definition makeMOV s dst (src: InstrArg s) :=
+Inductive MOVArg s :=
+| MOVArgR (r: GPReg s) :> MOVArg s 
+| MOVArgM a (m:MemSpec a) : MOVArg s
+| MOVArgI (v: VWORD s) :> MOVArg s.
+
+Coercion MOVArgM4 a (m: MemSpec a) : MOVArg OpSize4 := MOVArgM OpSize4 a m.
+
+Definition makeMOV s dst (src: MOVArg s) :=
   match dst, src with
-  | InstrArgR dst, InstrArgR src => MOVOP s (MovDstSrcRR s dst src)
-  | InstrArgR dst, InstrArgM a src => MOVOP s (MovDstSrcRM s a dst src)
-  | InstrArgR dst, InstrArgI n => MOVOP s (MovDstSrcRI s dst n)
-  | InstrArgM a dst, InstrArgR src => MOVOP s (MovDstSrcMR s a dst src)
-  | InstrArgM a dst, InstrArgI n => 
+  | MOVArgR dst, MOVArgR src => MOVOP s (MovDstSrcRR s dst src)
+  | MOVArgR dst, MOVArgM a src => MOVOP s (MovDstSrcRM s a dst src)
+  | MOVArgR dst, MOVArgI n => MOVOP s (MovDstSrcRI s dst n)
+  | MOVArgM a dst, MOVArgR src => MOVOP s (MovDstSrcMR s a dst src)
+  | MOVArgM a dst, MOVArgI n => 
     if VWORDasIMM s n is Some v then MOVOP s (MovDstSrcMI s a dst v) 
     else BADINSTR
   | _, _=> BADINSTR
@@ -217,46 +373,90 @@ Definition makeMOV s dst (src: InstrArg s) :=
 
 Notation "'MOV' x , y" := (makeMOV _ x%ms y%ms) (x,y at level 55, at level 60) : instr_scope.
 Notation "'MOV' 'BYTE' 'PTR' x , y" :=
-  (makeMOV OpSize1 x%ms y) (x,y at level 55, at level 60) : instr_scope.
+  (makeMOV OpSize1 (MOVArgM _ _ x%ms) y) (x,y at level 55, at level 60) : instr_scope.
 Notation "'MOV' 'WORD' 'PTR' x , y" :=
-  (makeMOV OpSize2 x%ms y) (x,y at level 55, at level 60) : instr_scope.
+  (makeMOV OpSize2 (MOVArgM _ _ x%ms) y) (x,y at level 55, at level 60) : instr_scope.
 Notation "'MOV' 'DWORD' 'PTR' x , y" :=
-  (makeMOV OpSize4 x%ms y) (x,y at level 55, at level 60) : instr_scope.
+  (makeMOV OpSize4 (MOVArgM _ _ x%ms) y) (x,y at level 55, at level 60) : instr_scope.
 Notation "'MOV' 'QWORD' 'PTR' x , y" :=
-  (makeMOV OpSize8 x%ms y) (x,y at level 55, at level 60) : instr_scope.
+  (makeMOV OpSize8 (MOVArgM _ _ x%ms) y) (x,y at level 55, at level 60) : instr_scope.
 
-(*---------------------------------------------------------------------------
-    MOV operations
-  ---------------------------------------------------------------------------*)
-
-Notation "'TEST' x , y"       := (TESTOP _  x%ms y) (x,y at level 55, at level 60) : instr_scope.
-Notation "'TEST' 'BYTE' 'PTR' x , y":= (TESTOP OpSize1 x%ms y) (x,y at level 55, at level 60) : instr_scope.
-Notation "'TEST' 'WORD' 'PTR' x , y":= (TESTOP OpSize2 x%ms y) (x,y at level 55, at level 60) : instr_scope.
-Notation "'TEST' 'DWORD 'PTR' x , y":= (TESTOP OpSize4 x%ms y) (x,y at level 55, at level 60) : instr_scope.
-Notation "'TEST' 'QWORD' 'PTR' x , y":= (TESTOP OpSize8 x%ms y) (x,y at level 55, at level 60) : instr_scope.
+Notation "'MOV' x , 'BYTE' 'PTR' y" :=
+  (makeMOV OpSize1 x (MOVArgM _ _ y%ms)) (x,y at level 55, at level 60) : instr_scope.
+Notation "'MOV' x , 'WORD' 'PTR' y" :=
+  (makeMOV OpSize2 x (MOVArgM _ _ y%ms)) (x,y at level 55, at level 60) : instr_scope.
+Notation "'MOV' x , 'DWORD' 'PTR' y" :=
+  (makeMOV OpSize4 x (MOVArgM _ _ y%ms)) (x,y at level 55, at level 60) : instr_scope.
+Notation "'MOV' x , 'QWORD' 'PTR' y" :=
+  (makeMOV OpSize8 x (MOVArgM _ _ y%ms)) (x,y at level 55, at level 60) : instr_scope.
 
 Notation "'MOVZX' x , y" := (MOVX OpSize1 OpSize4 x%ms y%ms) (x,y at level 55, at level 60) : instr_scope.
 Notation "'MOVSX' x , y" := (MOVX OpSize4 OpSize4 x%ms y%ms) (x,y at level 55, at level 60) : instr_scope.
+
+Example exMOV1 := MOV EDI, [ESI].
+Example exMOV2 := MOV BYTE PTR [EBX], (3:BYTE).
+Example exMOV3 (a:DWORD) := MOV EDI, a.
+Example exMOV4 (a:QWORD) := MOV RDI, a. 
+Example exMOV5 r := MOV AL, r.
+Example exMOV6 := MOV DX, BP. 
+
+(*---------------------------------------------------------------------------
+    TEST operations
+  ---------------------------------------------------------------------------*)
+
+Notation "'TEST' x , y"       := (TESTOP _  x%ms y) (x,y at level 55, at level 60) : instr_scope.
+Notation "'TEST' 'BYTE' 'PTR' x , y":= (TESTOP OpSize1 (RegMemM _ _ x%ms) y) (x,y at level 55, at level 60) : instr_scope.
+Notation "'TEST' 'WORD' 'PTR' x , y":= (TESTOP OpSize2 (RegMemM _ _ x%ms) y) (x,y at level 55, at level 60) : instr_scope.
+Notation "'TEST' 'DWORD 'PTR' x , y":= (TESTOP OpSize4 (RegMemM _ _ x%ms) y) (x,y at level 55, at level 60) : instr_scope.
+Notation "'TEST' 'QWORD' 'PTR' x , y":= (TESTOP OpSize8 (RegMemM _ _ x%ms) y) (x,y at level 55, at level 60) : instr_scope.
+
+Example exTEST1 := TEST AX, BX.
+Example exTEST2 := TEST BYTE PTR [EBX+4], AL.
+Example exTEST3 := TEST AL, (#2:IMM OpSize1).
 
 (*---------------------------------------------------------------------------
     Shift and rotate
   ---------------------------------------------------------------------------*)
 
 Notation "'SAL' x , c" := (SHIFTOP _ OP_SAL x%ms (ShiftCountI c)) (x, c at level 55, at level 60) : instr_scope.
+Notation "'SAL' x , 'CL'" := (SHIFTOP _ OP_SAL x%ms (ShiftCountCL)) (x at level 55, at level 60) : instr_scope.
 Notation "'SAR' x , c" := (SHIFTOP _ OP_SAR x%ms (ShiftCountI c)) (x, c at level 55, at level 60) : instr_scope.
+Notation "'SAR' x , 'CL'" := (SHIFTOP _ OP_SAR x%ms (ShiftCountCL)) (x at level 55, at level 60) : instr_scope.
 Notation "'SHL' x , c" := (SHIFTOP _ OP_SHL x%ms (ShiftCountI c)) (x, c at level 55, at level 60) : instr_scope.
+Notation "'SHL' x , 'CL'" := (SHIFTOP _ OP_SHL x%ms (ShiftCountCL)) (x at level 55, at level 60) : instr_scope.
 Notation "'SHR' x , c" := (SHIFTOP _ OP_SHR x%ms (ShiftCountI c)) (x, c at level 55, at level 60) : instr_scope.
+Notation "'SHR' x , 'CL'" := (SHIFTOP _ OP_SHR x%ms (ShiftCountCL)) (x at level 55, at level 60) : instr_scope.
 Notation "'RCL' x , c" := (SHIFTOP _ OP_RCL x%ms (ShiftCountI c)) (x, c at level 55, at level 60) : instr_scope.
+Notation "'RCL' x , 'CL'" := (SHIFTOP _ OP_RCL x%ms (ShiftCountCL)) (x at level 55, at level 60) : instr_scope.
 Notation "'RCR' x , c" := (SHIFTOP _ OP_RCR x%ms (ShiftCountI c)) (x, c at level 55, at level 60) : instr_scope.
+Notation "'RCR' x , 'CL'" := (SHIFTOP _ OP_RCR x%ms (ShiftCountCL)) (x at level 55, at level 60) : instr_scope.
 Notation "'ROL' x , c" := (SHIFTOP _ OP_ROL x%ms (ShiftCountI c)) (x, c at level 55, at level 60) : instr_scope.
+Notation "'ROL' x , 'CL'" := (SHIFTOP _ OP_ROL x%ms (ShiftCountCL)) (x at level 55, at level 60) : instr_scope.
 Notation "'ROR' x , c" := (SHIFTOP _ OP_ROR x%ms (ShiftCountI c)) (x, c at level 55, at level 60) : instr_scope.
+Notation "'ROR' x , 'CL'" := (SHIFTOP _ OP_ROR x%ms (ShiftCountCL)) (x at level 55, at level 60) : instr_scope.
+
+Example exSAL1 := SAL EAX, CL.
+Example exRCL1 := RCL [ESI + 4], 5.
 
 Notation "'IMUL' x , y" := (IMUL x%ms y%ms) (x,y at level 55, at level 60) : instr_scope.
 
-Notation "'LEA' x , y" := (makeLEA _ x y%ms) (x,y at level 55, at level 60) : instr_scope.
+(*---------------------------------------------------------------------------
+    LEA
+  ---------------------------------------------------------------------------*)
+Notation "'LEA' x , y" := (instr.LEA _ x (RegMemM _ _ y%ms)) (x,y at level 55, at level 60) : instr_scope.
+Example exLEA1 := LEA EAX, [EBX + ESI*8 + 24].
+Example exLEA2 := LEA R12, [R14 + RSI*4].
 
-Notation "'RET' x" := (RETOP x) (at level 60, x at level 55, format "'RET' x") : instr_scope.
+(*---------------------------------------------------------------------------
+    RET
+  ---------------------------------------------------------------------------*)
+Notation "'RET' x" := (RETOP x) (at level 60, x at level 55) : instr_scope.
+Example exRET1 := RET 12.
+Example exRET2 := RET 0.
 
+(*---------------------------------------------------------------------------
+    IN/OUT
+  ---------------------------------------------------------------------------*)
 Notation "'OUT' 'DX' ',' 'AL'" := (OUTOP OpSize1 PortDX) : instr_scope.
 Notation "'OUT' 'DX' ',' 'EAX'" := (OUTOP OpSize4 PortDX) : instr_scope.
 Notation "'IN'  'DX' ',' 'AL'" := (INOP OpSize1 PortDX) : instr_scope.
@@ -275,25 +475,3 @@ Arguments POP (dst)%ms.
 (* Typical use: in "Eval showinstr in linearize p" *)
 Declare Reduction showinstr := cbv beta delta -[fromNat makeMOV makeBOP] zeta iota.
 
-Module Examples.
-Open Scope instr_scope.
-
-Example ex1 := ADD EAX, [EBX + 3].
-Example ex2 := INC BYTE PTR [ECX + EDI*4 + 78].
-Example ex2' := INC DWORD PTR [ECX + EDI*4 + 78].
-Example ex3 (r:NonSPReg32) := MOV EDI, [r].
-Example ex4 (a:DWORD) := MOV EDI, [ESI]. 
-Example ex4' (a:DWORD) := MOV BYTE PTR [EBX], natAsBYTE 3.
-Example ex5 (a:DWORD) := MOV EDI, a.
-Example ex5' (a:QWORD) := MOV RDI, a. 
-Example ex11 := CMP BYTE PTR [EDI + ECX*2], #c"*".
-Example ex13 := LEA EBP, FS:[RBP + 23].
-Example ex6 r := MOV AL, r.
-Example ex12 := INC BX.
-(*Example ex7 (r:NonSPReg64) := POP [r + #x"0000001C"].*)
-Example ex8 := CMP AL, #c"!".
-Example ex9 := MOV DX, BP. 
-Example ex10 := NOT DWORD PTR [EBX + EDI*4 + 3]. 
-
-Close Scope instr_scope.
-End Examples.
